Generalize addr_restrictions

theories/linking.v
@@ -6,10 +6,8 @@ From cap_machine Require Import addr_reg machine_base.
 
 Section Linking.
 
-  Variable b_stk: Addr.
-  Variable e_stk: Addr.
-  Variable stk_pos: (b_stk < e_stk)%a.
-
+  (** Symbols are used to identify imported/exported word (often capabilites)
+      They can be of any type with decidable equality *)
   Variable Symbols: Type.
   Variable Symbols_eq_dec: EqDecision Symbols.
   Variable Symbols_countable: Countable Symbols.
@@ -25,9 +23,54 @@ Section Linking.
       word_restrictions w dom1 ->
       word_restrictions w dom2.
 
-  Notation imports_type := (gset (Symbols * Addr)).
-  Notation exports_type := (gmap Symbols Word).
-  Notation segment_type := (gmap Addr Word).
+  (** Example of a word_restrictions, ensure all capabilites point
+      into the given segment *)
+  Example can_address_only (word: Word) (addr_set: gset Addr) :=
+    match word with
+    | WInt _ => True
+    | WCap _ b e _ => ∀ a, (b <= a < e)%a -> a ∈ addr_set
+    end.
+  Lemma can_address_only_incr :
+    forall w dom1 dom2,
+      dom1 ⊆ dom2 ->
+      can_address_only w dom1 ->
+      can_address_only w dom2.
+  Proof.
+    intros w dom1 dom2 dom1_dom2.
+    destruct w. auto.
+    intros ca_dom1 addr addr_in_be.
+    apply dom1_dom2. apply (ca_dom1 addr addr_in_be).
+  Qed.
+
+  (** A predicate that can be used to restrict the address space to a subsection
+      of memory (ex: reserve space for a stack).
+      This should remain true on the link (union of segments where it holds) *)
+  Variable addr_restrictions: gset Addr -> Prop.
+  Variable addr_restrictions_union_stable:
+    forall dom1 dom2,
+      addr_restrictions dom1 ->
+      addr_restrictions dom2 ->
+      addr_restrictions (dom1 ∪ dom2).
+
+  (** Example addr_restriction, address greater than a given end_stack parameter *)
+  Example addr_gt_than (e_stk: Addr) (dom: gset Addr) :=
+    forall a, a ∈ dom -> (e_stk < a)%a.
+  Lemma addr_gt_than_union_stable (e_stk: Addr) :
+    forall dom1 dom2,
+      addr_gt_than e_stk dom1 ->
+      addr_gt_than e_stk dom2 ->
+      addr_gt_than e_stk (dom1 ∪ dom2).
+  Proof.
+    intros dom1 dom2 gt_dom1 gt_dom2 a a_in_1or2.
+    apply elem_of_union in a_in_1or2.
+    destruct a_in_1or2 as [ a_in_1 | a_in_2 ].
+    apply (gt_dom1 a a_in_1).
+    apply (gt_dom2 a a_in_2).
+  Qed.
+
+  Definition imports_type := (gset (Symbols * Addr)).
+  Definition exports_type := (gmap Symbols Word).
+  Definition segment_type := (gmap Addr Word).
 
   Record pre_component := {
     segment : segment_type;
@@ -51,7 +94,8 @@ Section Linking.
         (Hwr_exp: ∀ s w, pcomp.(exports) !! s = Some w -> word_restrictions w (dom _ pcomp.(segment)))
         (Himp: ∀ s a, (s, a) ∈ pcomp.(imports) -> is_Some (pcomp.(segment) !! a))
         (Himpdisj: ∀ s1 s2 a, (s1, a) ∈ pcomp.(imports) -> (s2, a) ∈ pcomp.(imports) -> s1 = s2)
-        (Hwr_ms: ∀ a w, pcomp.(segment) !! a = Some w -> word_restrictions w (dom _ pcomp.(segment))),
+        (Hwr_ms: ∀ a w, pcomp.(segment) !! a = Some w -> word_restrictions w (dom _ pcomp.(segment)))
+        (Har_ms: addr_restrictions (dom _ pcomp.(segment))),
         well_formed_pre_comp pcomp.
 
   Inductive well_formed_comp: component -> Prop :=
@@ -72,145 +116,163 @@ Section Linking.
         (Hwfcomp: well_formed_comp (Main pcomp w_main)),
         is_program (Main pcomp w_main).
 
-  (** Add values defined in exp to the segment
-      at addresses specified in imp *)
-  Definition resolve_imports
-     (imp: imports_type) (exp: exports_type) (ms: segment_type) :=
-    set_fold (fun '(s, a) m => match exp !! s with
-      | Some w => <[a:=w]> m
-      | None => m end) ms imp.
+  Section resolve_imports.
+    (** Add values defined in exp to the segment
+        at addresses specified in imp *)
+    Definition resolve_imports
+      (imp: imports_type) (exp: exports_type) (ms: segment_type) :=
+      set_fold (fun '(s, a) m => match exp !! s with
+        | Some w => <[a:=w]> m
+        | None => m end) ms imp.
 
-  Lemma resolve_imports_spec:
-    forall imp exp ms a
-      (Himpdisj: forall s1 s2 a, (s1, a) ∈ imp -> (s2, a) ∈ imp -> s1 = s2),
-      ((~ exists s, (s, a) ∈ imp) ->
-       (resolve_imports imp exp ms) !! a = ms !! a) /\
-      (forall s, (s, a) ∈ imp ->
-       (exp !! s = None /\ (resolve_imports imp exp ms) !! a = ms !! a) \/ (exists wexp, exp !! s = Some wexp /\ (resolve_imports imp exp ms) !! a = Some wexp)).
-  Proof.
-    intros imp exp ms a. eapply (set_fold_ind_L (fun m imp => (forall s1 s2 a, (s1, a) ∈ imp -> (s2, a) ∈ imp -> s1 = s2) -> ((~ exists s, (s, a) ∈ imp) -> m !! a = ms !! a) /\ (forall s, (s, a) ∈ imp -> (exp !! s = None /\ m !! a = ms !! a) \/ (exists wexp, exp !! s = Some wexp /\ m !! a = Some wexp))) (fun '(s, a) m => match exp !! s with Some w => <[a:=w]> m | None => m end)); eauto.
-    { intros. split; auto. intros.
-      eapply elem_of_empty in H0; elim H0; auto. }
-    intros. destruct x. split.
-    { intros. destruct (exp !! s).
-      - rewrite lookup_insert_ne; auto.
-        + apply H0.
-          * intros. eapply H1; eapply elem_of_union; right; eauto.
-          * intro Y. destruct Y as [sy Hiny].
-            eapply H2. exists sy. eapply elem_of_union. right; eauto.
-        + intro. eapply H2. exists s.
-          eapply elem_of_union. left. eapply elem_of_singleton. rewrite H3. reflexivity.
-      - apply H0.
-        + intros. eapply H1; eapply elem_of_union; right; eauto.
-        + intro Y. destruct Y as [sy Hiny].
-          eapply H2. exists sy. eapply elem_of_union. right; auto. }
-    { intros; destruct (exp !! s) eqn:Hexp.
-      - destruct (addr_eq_dec a f) as [eq | neq].
-        + rewrite eq. rewrite lookup_insert.
-          right. assert (s0 = s) as ->; eauto.
-          eapply elem_of_union in H2. destruct H2.
-          * generalize (proj1 (elem_of_singleton _ _) H2). inversion 1; subst; auto.
-          * eapply (H1 s0 s a); [eapply elem_of_union_r; auto|eapply elem_of_union_l; eapply elem_of_singleton; eauto].
-            rewrite eq. reflexivity.
-        + rewrite lookup_insert_ne; auto.
-          eapply elem_of_union in H2; destruct H2.
-          * erewrite elem_of_singleton in H2. inversion H2; congruence.
-          * eapply H0; auto.
-            intros; eapply H1; eapply elem_of_union; right; eauto.
-      - eapply elem_of_union in H2. destruct H2.
-        + erewrite elem_of_singleton in H2. inversion H2; subst; clear H2.
-          left; split; auto. eapply (proj1 (H0 ltac:(intros; eapply H1; eapply elem_of_union; right; eauto))).
-          intro Y. destruct Y as [sy Hsy].
-          eapply H. replace s with sy; auto.
-          eapply H1; [eapply elem_of_union_r; eauto| eapply elem_of_union_l; eapply elem_of_singleton; eauto].
-        + eapply H0; auto.
-          intros; eapply H1; eapply elem_of_union_r; eauto. }
-  Qed.
+    Lemma resolve_imports_spec:
+      forall imp exp ms a
+        (Himpdisj: forall s1 s2 a, (s1, a) ∈ imp -> (s2, a) ∈ imp -> s1 = s2),
+        ((~ exists s, (s, a) ∈ imp) ->
+        (resolve_imports imp exp ms) !! a = ms !! a) /\
+        (forall s, (s, a) ∈ imp ->
+        (exp !! s = None /\ (resolve_imports imp exp ms) !! a = ms !! a) \/ (exists wexp, exp !! s = Some wexp /\ (resolve_imports imp exp ms) !! a = Some wexp)).
+    Proof.
+      intros imp exp ms a. eapply (set_fold_ind_L (fun m imp => (forall s1 s2 a, (s1, a) ∈ imp -> (s2, a) ∈ imp -> s1 = s2) -> ((~ exists s, (s, a) ∈ imp) -> m !! a = ms !! a) /\ (forall s, (s, a) ∈ imp -> (exp !! s = None /\ m !! a = ms !! a) \/ (exists wexp, exp !! s = Some wexp /\ m !! a = Some wexp))) (fun '(s, a) m => match exp !! s with Some w => <[a:=w]> m | None => m end)); eauto.
+      { intros. split; auto. intros.
+        eapply elem_of_empty in H0; elim H0; auto. }
+      intros. destruct x. split.
+      { intros. destruct (exp !! s).
+        - rewrite lookup_insert_ne; auto.
+          + apply H0.
+            * intros. eapply H1; eapply elem_of_union; right; eauto.
+            * intro Y. destruct Y as [sy Hiny].
+              eapply H2. exists sy. eapply elem_of_union. right; eauto.
+          + intro. eapply H2. exists s.
+            eapply elem_of_union. left. eapply elem_of_singleton. rewrite H3. reflexivity.
+        - apply H0.
+          + intros. eapply H1; eapply elem_of_union; right; eauto.
+          + intro Y. destruct Y as [sy Hiny].
+            eapply H2. exists sy. eapply elem_of_union. right; auto. }
+      { intros; destruct (exp !! s) eqn:Hexp.
+        - destruct (addr_eq_dec a f) as [eq | neq].
+          + rewrite eq. rewrite lookup_insert.
+            right. assert (s0 = s) as ->; eauto.
+            eapply elem_of_union in H2. destruct H2.
+            * generalize (proj1 (elem_of_singleton _ _) H2). inversion 1; subst; auto.
+            * eapply (H1 s0 s a); [eapply elem_of_union_r; auto|eapply elem_of_union_l; eapply elem_of_singleton; eauto].
+              rewrite eq. reflexivity.
+          + rewrite lookup_insert_ne; auto.
+            eapply elem_of_union in H2; destruct H2.
+            * erewrite elem_of_singleton in H2. inversion H2; congruence.
+            * eapply H0; auto.
+              intros; eapply H1; eapply elem_of_union; right; eauto.
+        - eapply elem_of_union in H2. destruct H2.
+          + erewrite elem_of_singleton in H2. inversion H2; subst; clear H2.
+            left; split; auto. eapply (proj1 (H0 ltac:(intros; eapply H1; eapply elem_of_union; right; eauto))).
+            intro Y. destruct Y as [sy Hsy].
+            eapply H. replace s with sy; auto.
+            eapply H1; [eapply elem_of_union_r; eauto| eapply elem_of_union_l; eapply elem_of_singleton; eauto].
+          + eapply H0; auto.
+            intros; eapply H1; eapply elem_of_union_r; eauto. }
+    Qed.
 
-  (** Resolve imports of an address in imports is either
-      - unchanged if the address are in not in the exports
-      - the exported value if it is in exports *)
-  Lemma resolve_imports_spec_in:
-    forall imp exp ms a s
-      (Himpdisj: forall s1 s2 a, (s1, a) ∈ imp -> (s2, a) ∈ imp -> s1 = s2),
-      (s, a) ∈ imp ->
-      (exp !! s = None /\ (resolve_imports imp exp ms) !! a = ms !! a) \/
-      (exists wexp, exp !! s = Some wexp /\ (resolve_imports imp exp ms) !! a = Some wexp).
-  Proof.
-    intros. eapply resolve_imports_spec; eauto.
-  Qed.
+    (** Resolve imports of an address in imports is either
+        - unchanged if the address are in not in the exports
+        - the exported value if it is in exports *)
+    Lemma resolve_imports_spec_in:
+      forall imp exp ms a s
+        (Himpdisj: forall s1 s2 a, (s1, a) ∈ imp -> (s2, a) ∈ imp -> s1 = s2),
+        (s, a) ∈ imp ->
+        (exp !! s = None /\ (resolve_imports imp exp ms) !! a = ms !! a) \/
+        (exists wexp, exp !! s = Some wexp /\ (resolve_imports imp exp ms) !! a = Some wexp).
+    Proof.
+      intros. eapply resolve_imports_spec; eauto.
+    Qed.
 
-  (** Resolve imports does not change addresses not in imports *)
-  Lemma resolve_imports_spec_not_in:
-    forall imp exp ms a
-      (Himpdisj: forall s1 s2 a, (s1, a) ∈ imp -> (s2, a) ∈ imp -> s1 = s2),
-      ((~ exists s, (s, a) ∈ imp) ->
-       (resolve_imports imp exp ms) !! a = ms !! a).
-  Proof.
-    intros. eapply resolve_imports_spec; eauto.
-  Qed.
+    (** Resolve imports does not change addresses not in imports *)
+    Lemma resolve_imports_spec_not_in:
+      forall imp exp ms a
+        (Himpdisj: forall s1 s2 a, (s1, a) ∈ imp -> (s2, a) ∈ imp -> s1 = s2),
+        ((~ exists s, (s, a) ∈ imp) ->
+        (resolve_imports imp exp ms) !! a = ms !! a).
+    Proof.
+      intros. eapply resolve_imports_spec; eauto.
+    Qed.
 
-  (** A address from resolve imports contains either:
-      - an added export
-      - an original memory segment value *)
-  Lemma resolve_imports_spec_simple :
-    forall imp exp ms a w
-      (Himpdisj: forall s1 s2 a, (s1, a) ∈ imp -> (s2, a) ∈ imp -> s1 = s2),
-      (resolve_imports imp exp ms) !! a = Some w ->
-        (∃ s, exp !! s = Some w) \/ (ms !! a = Some w).
-  Proof.
-    intros imp exp ms a w Himpdisj.
-    apply (set_fold_ind_L (
-      fun ms' imp' =>
-        ms' !! a = Some w ->
-        (∃ s, exp !! s = Some w) \/ (ms !! a = Some w))).
-    auto.
-    intros [s a'] imps' ms' _ Hind.
-    destruct (Some_dec (exp !! s)) as [ [w' ex_w] | ex_w ];
-    rewrite ex_w.
-    - destruct (decide (a' = a)) as [ aa' | aa']. rewrite <- aa'.
-      + rewrite lookup_insert. intros ww'. rewrite ww' in ex_w.
-        left. exists s. apply ex_w.
-      + rewrite (lookup_insert_ne _ _ _ _ aa'). apply Hind.
-    - apply Hind.
-  Qed.
+    (** A address from resolve imports contains either:
+        - an added export
+        - an original memory segment value *)
+    Lemma resolve_imports_spec_simple :
+      forall imp exp ms a w
+        (Himpdisj: forall s1 s2 a, (s1, a) ∈ imp -> (s2, a) ∈ imp -> s1 = s2),
+        (resolve_imports imp exp ms) !! a = Some w ->
+          (∃ s, exp !! s = Some w) \/ (ms !! a = Some w).
+    Proof.
+      intros imp exp ms a w Himpdisj.
+      apply (set_fold_ind_L (
+        fun ms' imp' =>
+          ms' !! a = Some w ->
+          (∃ s, exp !! s = Some w) \/ (ms !! a = Some w))).
+      auto.
+      intros [s a'] imps' ms' _ Hind.
+      destruct (Some_dec (exp !! s)) as [ [w' ex_w] | ex_w ];
+      rewrite ex_w.
+      - destruct (decide (a' = a)) as [ aa' | aa']. rewrite <- aa'.
+        + rewrite lookup_insert. intros ww'. rewrite ww' in ex_w.
+          left. exists s. apply ex_w.
+        + rewrite (lookup_insert_ne _ _ _ _ aa'). apply Hind.
+      - apply Hind.
+    Qed.
 
-  (** Resolve imports increases the domain of the memory segment *)
-  Lemma resolve_imports_dom :
-    forall imp exp ms,
-      dom (gset Addr) ms ⊆ dom (gset Addr) (resolve_imports imp exp ms).
-  Proof.
-    intros imp exp ms a a_in_ms.
-    apply (set_fold_ind_L (fun ms imp => a ∈ dom _ ms)).
-    - apply a_in_ms.
-    - intros. destruct x as [s a0]. destruct (exp !! s).
-      apply dom_insert_subseteq. apply H0.
-      apply H0.
-  Qed.
+    (** Resolve imports increases the domain of the memory segment *)
+    Lemma resolve_imports_dom :
+      forall imp exp ms,
+        dom (gset Addr) ms ⊆ dom (gset Addr) (resolve_imports imp exp ms).
+    Proof.
+      intros imp exp ms a a_in_ms.
+      apply (set_fold_ind_L (fun ms imp => a ∈ dom _ ms)).
+      - apply a_in_ms.
+      - intros. destruct x as [s a0]. destruct (exp !! s).
+        apply dom_insert_subseteq. apply H0.
+        apply H0.
+    Qed.
 
-  Lemma resolve_imports_dom_rev :
-    forall imp exp ms a,
-      a ∈ dom (gset Addr) (resolve_imports imp exp ms) ->
-      a ∈ dom (gset Addr) ms \/ ∃ s, (s,a) ∈ imp.
-  Proof.
-    intros imp exp ms a.
-    apply (set_fold_ind_L (
-      fun ms' imp' =>
-        a ∈ dom (gset Addr) ms' ->
-        a ∈ dom (gset Addr) ms \/ ∃ s, (s,a) ∈ imp')).
-    auto.
-    intros [s a'] imps' ms' sa'_notin_imps' Hind.
-    destruct (Some_dec (exp !! s)) as [ [w' ex_w] | ex_w ];
-    rewrite ex_w.
-    - destruct (decide (a' = a)) as [ aa' | aa']. rewrite <- aa'.
-      + right. exists s. apply elem_of_union_l, elem_of_singleton. reflexivity.
-      + rewrite elem_of_dom. rewrite (lookup_insert_ne _ _ _ _ aa').
-        rewrite <- elem_of_dom. intros a_in_ms'.
-        destruct (Hind a_in_ms') as [H | [s' H]].
+    Lemma resolve_imports_dom_rev :
+      forall imp exp ms a,
+        a ∈ dom (gset Addr) (resolve_imports imp exp ms) ->
+        a ∈ dom (gset Addr) ms \/ ∃ s, (s,a) ∈ imp.
+    Proof.
+      intros imp exp ms a.
+      apply (set_fold_ind_L (
+        fun ms' imp' =>
+          a ∈ dom (gset Addr) ms' ->
+          a ∈ dom (gset Addr) ms \/ ∃ s, (s,a) ∈ imp')).
+      auto.
+      intros [s a'] imps' ms' sa'_notin_imps' Hind.
+      destruct (Some_dec (exp !! s)) as [ [w' ex_w] | ex_w ];
+      rewrite ex_w.
+      - destruct (decide (a' = a)) as [ aa' | aa']. rewrite <- aa'.
+        + right. exists s. apply elem_of_union_l, elem_of_singleton. reflexivity.
+        + rewrite elem_of_dom. rewrite (lookup_insert_ne _ _ _ _ aa').
+          rewrite <- elem_of_dom. intros a_in_ms'.
+          destruct (Hind a_in_ms') as [H | [s' H]].
+          left. apply H. right. exists s'. apply elem_of_union_r, H.
+      - intros a_in_ms'. destruct (Hind a_in_ms') as [H | [s' H]].
         left. apply H. right. exists s'. apply elem_of_union_r, H.
-    - intros a_in_ms'. destruct (Hind a_in_ms') as [H | [s' H]].
-      left. apply H. right. exists s'. apply elem_of_union_r, H.
-  Qed.
+    Qed.
+
+    Lemma resolve_imports_dom_eq :
+      forall imp exp ms,
+        (∀ s a, (s,a) ∈ imp -> is_Some (ms !! a)) ->
+        dom (gset Addr) (resolve_imports imp exp ms) = dom (gset Addr) ms.
+    Proof.
+      intros imp exp ms imp_issome.
+      apply (anti_symm _).
+      - intros a a_in_ri.
+        destruct (resolve_imports_dom_rev imp exp ms a a_in_ri) as [a_in_ms | [s sa_in_imps]].
+        assumption.
+        rewrite elem_of_dom.
+        apply (imp_issome s a sa_in_imps).
+      - apply resolve_imports_dom.
+    Qed.
+
+  End resolve_imports.
 
   Definition opt_merge_fun {T:Type} (o1 o2: option T) :=
     match o1 with
@@ -394,8 +456,8 @@ Section Linking.
       (Hms_disj: pcomp1.(segment) ##ₘ pcomp2.(segment)) :
       well_formed_pre_comp (link_pre_comp pcomp1 pcomp2).
     Proof.
-      inversion wf_1 as [pcomp1' Hdisj1 Hexp1 Himp1 Himpdisj1 Hnpwl1 Hdisjstk1].
-      inversion wf_2 as [pcomp2' Hdisj2 Hexp2 Himp2 Himpdisj2 Hnpwl2 Hdisjstk2].
+      inversion wf_1 as [pcomp1' Hdisj1 Hexp1 Himp1 Himpdisj1 Hwr_ms1 Har_ms1].
+      inversion wf_2 as [pcomp2' Hdisj2 Hexp2 Himp2 Himpdisj2 Hwr_ms2 Har_ms2].
       apply wf_pre_intro.
       + intros s is_some_s. (* exports are disjoint from import *)
         specialize (Hdisj1 s). specialize (Hdisj2 s).
@@ -438,8 +500,8 @@ Section Linking.
           rewrite (map_disjoint_Some_r pcomp1.(segment) pcomp2.(segment) _ _ Hms_disj ms2a) in s2_a_in_imp1.
           contradiction (is_Some_None s2_a_in_imp1).
         - apply (Himpdisj2 s1 s2 a s1_a_in_imp2 s2_a_in_imp2).
-      + intros a w ms_a_w. (* HERE *)
-        specialize (Hnpwl1 a w). specialize (Hnpwl2 a w).
+      + intros a w ms_a_w.
+        specialize (Hwr_ms1 a w). specialize (Hwr_ms2 a w).
         destruct (resolve_imports_spec_simple _ _ _ _ _ Himpdisj2 ms_a_w) as [[ s exp_s_w ] | ms_a_w'].
         destruct (opt_merge_l_or_r exp_s_w) as [exp1_s | exp2_s].
         apply (word_restrictions_incr _ _ _ resolve_imports_dom_dom1 (Hexp1 s w exp1_s)).
@@ -450,21 +512,24 @@ Section Linking.
         apply (word_restrictions_incr _ _ _ resolve_imports_dom_dom2 (Hexp2 s w exp2_s)).
         apply lookup_union_Some in ms_a_w''.
         destruct ms_a_w'' as [ms1_a_w | ms2_a_w].
-        apply (word_restrictions_incr _ _ _ resolve_imports_dom_dom1 (Hnpwl1 ms1_a_w)).
-        apply (word_restrictions_incr _ _ _ resolve_imports_dom_dom2 (Hnpwl2 ms2_a_w)).
+        apply (word_restrictions_incr _ _ _ resolve_imports_dom_dom1 (Hwr_ms1 ms1_a_w)).
+        apply (word_restrictions_incr _ _ _ resolve_imports_dom_dom2 (Hwr_ms2 ms2_a_w)).
         apply Hms_disj.
-      (* + intros a a_in_ri.
-        destruct (resolve_imports_dom_rev _ _ _ a a_in_ri) as [a_in_ri' | [s sa_in_imp2]].
-        destruct (resolve_imports_dom_rev _ _ _ a a_in_ri') as [a_in_ri'' | [s sa_in_imp1]].
-        apply dom_union, elem_of_union in a_in_ri''.
-        destruct a_in_ri'' as [a_in_ms1 | a_in_ms2].
-        eauto using Hdisjstk1. eauto using Hdisjstk2.
-        specialize (Himp1 _ _ sa_in_imp1).
-        apply elem_of_dom in Himp1.
-        eauto using Hdisjstk1.
-        specialize (Himp2 _ _ sa_in_imp2).
-        apply elem_of_dom in Himp2.
-        eauto using Hdisjstk2. *)
+      + rewrite resolve_imports_dom_eq.
+        rewrite resolve_imports_dom_eq.
+        assert (Hdom: dom (gset Addr) (map_union (segment pcomp1) (segment pcomp2)) = dom _ (segment pcomp1) ∪ dom _ (segment pcomp2)).
+        { apply (anti_symm _); rewrite dom_union; reflexivity. }
+        rewrite Hdom. clear Hdom.
+        apply addr_restrictions_union_stable; assumption.
+        intros s a sa_in_imps1.
+        apply elem_of_dom. rewrite dom_union.
+        apply elem_of_union_l. rewrite elem_of_dom.
+        apply (Himp1 s a sa_in_imps1).
+        intros s a sa_in_imps2.
+        apply elem_of_dom.
+        apply resolve_imports_dom. rewrite dom_union.
+        apply elem_of_union_r. rewrite elem_of_dom.
+        apply (Himp2 s a sa_in_imps2).
     Qed.
 
     (** mlink_main_lib forms a link from a main and a lib *)
